LambdaLetDollar.v
@@ -468,10 +468,27 @@ Global Hint Constructors contr' : core.
 
 Reserved Notation "e1 -->' e2" (at level 40).
 Inductive step' : tm' ␀ → tm' ␀ → Prop :=
-| step_tm' : ∀ k t e1 e2, <| k[t[e1]] |> -->' <| k[t[e2]] |>
+| step_tm' : ∀ (k : K' ␀) (t : T' ␀) (e1 e2 : tm' ␀), e1 ~>' e2 → <| k[t[e1]] |> -->' <| k[t[e2]] |>
 where "e1 -->' e2" := (step' e1 e2).
+Global Hint Constructors step' : core.
 
 Notation "e1 -->'* e2" := (multi step' e1 e2) (at level 40).
+
+Lemma contr_is_step' : ∀ e1 e2,
+  e1 ~>' e2 → e1 -->' e2.
+Proof.
+  intros.
+  apply (step_tm' K_nil' T_nil' e1 e2).
+  assumption.
+Qed.
+Definition contr_beta' : ∀ e (v : val' ␀), <| (λ e) v |> ~>' <| e [ 0 := v ] |> := λ e v, contr_tm' (redex_beta' (val_abs' e) v).
+Definition contr_dollar' : ∀ (v1 v2 : val' ␀), <| v1 $ v2 |> ~>' <| v1 v2 |> := λ v1 v2, contr_tm' (redex_dollar' v1 v2).
+Definition contr_shift' : ∀ (v : val' ␀) e, <| v $ S₀ e |> ~>' <| e [ 0 := v ] |> := λ v e, contr_tm' (redex_shift' v e).
+Definition contr_dol_let' : ∀ (v : val' ␀) e1 e2, <| v $ let S₀ e1 in e2 |> ~>' <| (λ {liftV' v} $ e2) $ S₀ e1 |> := λ v e1 e2, contr_tm' (redex_dol_let' v e1 e2).
+Definition contr_let' : ∀ (j : J' ␀) (p : non' ␀), <| j[p] |> ~>' <| let p in ↑j[0] |> := λ j p, contr_tm' (redex_let' j p).
+Definition contr_let_beta' : ∀ (v : val' ␀) e, <| let v in e |> ~>' <| e [ 0 := v ] |> := λ v e, contr_tm' (redex_let_beta' v e).
+Definition contr_let_assoc' : ∀ e1 e2 e3, <| let (let S₀ e1 in e2) in e3 |> ~>' <| let S₀ e1 in let e2 in ↑e3 |> := λ e1 e2 e3, contr_tm' (redex_let_assoc' e1 e2 e3).
+Global Hint Resolve contr_is_step' contr_beta' contr_dollar' contr_shift' contr_dol_let' contr_let' contr_let_beta' contr_let_assoc' : core.
 
 Fixpoint eval' i e :=
   match i with
@@ -528,3 +545,83 @@ Section Examples.
   Compute (decompose' (eval' 7 <| _id $ ej123 |>)).
   
 End Examples.
+
+
+Lemma plug_non_is_non' : ∀ (k' : K' ␀) (t' : T' ␀) (p' : non' ␀),
+  ∃ p'', <| k' [t' [p']] |> = non_to_tm' p''.
+Proof.
+  intros; destruct k'; cbn in *.
+  destruct t'; cbn in *.
+  eexists; reflexivity.
+  eexists (non_dol' _ _); reflexivity.
+  eexists (non_let' _ _); reflexivity.
+Qed.
+
+Lemma redex_is_non' : ∀ {A} r', ∃ p', @redex_to_term' A r' = non_to_tm' p'.
+Proof.
+  intros. destruct r'; cbn;
+  try solve [try destruct j; eexists (non_app' _ _) + eexists (non_dol' _ _) + eexists (non_let' _ _); reflexivity].
+Qed.
+
+Lemma non_when_contr' : ∀ e' e'',
+  e' ~>' e'' →
+  ∃ p', e' = non_to_tm' p'.
+Proof.
+  intros. inversion H; clear H; subst.
+  apply redex_is_non'.
+Qed.
+
+Lemma non_when_step' : ∀ e' e'',
+  e' -->' e'' →
+  ∃ p', e' = non_to_tm' p'.
+Proof.
+  intros. inversion H; clear H; subst.
+  apply non_when_contr' in H0 as [p' Hp]; subst.
+  apply plug_non_is_non'.
+Qed.
+
+Lemma non_when_steps_to_non' : ∀ e' (p'' : non' ␀),
+  e' -->'* p'' →
+  ∃ p', e' = non_to_tm' p'.
+Proof.
+  intros. dependent induction H. exists p''. reflexivity.
+  destruct (IHmulti p'') as [p' IH]; auto; subst.
+  apply (non_when_step' x p'); auto.
+Qed.
+
+Lemma non_when_steps_to_plug_non' : ∀ e (k' : K' ␀) (t' : T' ␀) (p' : non' ␀),
+  e -->'* <| k' [t' [p']] |> →
+  ∃ p, e = non_to_tm' p.
+Proof.
+  intros. destruct (plug_non_is_non' k' t' p') as [p'' Hp''].
+  apply (non_when_steps_to_non' _ p''). rewrite Hp'' in *. assumption.
+Qed.
+
+Lemma multi_contr' : ∀ e1 e2 e3,
+  e1 ~>' e2 →
+  e2 -->'* e3 →
+  e1 -->'* e3.
+Proof.
+  intros. eapply multi_step; try eapply (step_tm' K_nil' T_nil'); cbn; eassumption.
+Qed.
+
+Lemma step_let' : ∀ e1 e2 e,
+  e1 -->' e2 →
+  <| let e1 in e |> -->' <| let e2 in e |>.
+Proof.
+  intros. generalize dependent e.
+  induction H; auto; intros.
+  apply (step_tm' (K_let' k e) t e1 e2).
+  apply H.
+Qed.
+
+Lemma multi_let' : ∀ e1 e2 e,
+  e1 -->'* e2 →
+  <| let e1 in e |> -->'* <| let e2 in e |>.
+Proof.
+  intros. generalize dependent e.
+  induction H; auto; intros.
+  eapply (multi_step); [idtac | apply IHmulti].
+  apply step_let'.
+  apply H.
+Qed.
