LambdaDollarToLet.v
@@ -4,50 +4,108 @@ Require Export LambdaLetDollar.
 
 Reserved Notation "e ~ₑ e'" (at level 40).
 Reserved Notation "v ~ᵥ v'" (at level 40).
+Reserved Notation "p ~ₚ p'" (at level 40).
 Reserved Notation "j ~ⱼ j'" (at level 40).
 Reserved Notation "k ~ₖ k'" (at level 40).
+Reserved Notation "t ~ₜ t'" (at level 40).
 Inductive sim_J {A} : J A → J' A → Prop :=
 | sim_J_fun : ∀ e e', e ~ₑ e' → J_fun e ~ⱼ J_fun' e'
 | sim_J_arg : ∀ v v', v ~ᵥ v' → J_arg v ~ⱼ J_arg' v'
 | sim_J_dol : ∀ e e', e ~ₑ e' → J_dol e ~ⱼ J_dol' e'
+with sim_T {A} : T A → T' A → Prop :=
+| sim_T_nil  : T_nil ~ₜ T_nil'
+| sim_T_cons : ∀ v v' k k' t t', T_cons v k t ~ₜ T_cons' v' k' t'
 with sim_K {A} : K A → K' A → Prop :=
 | sim_K_nil  : K_nil ~ₖ K_nil'
 | sim_K_cons : ∀ j j' k k',
     j ~ⱼ j' → k ~ₖ k' →
-    K_cons j k ~ₖ K_let' k' (plugJ' (liftJ' j') <{ 0 }>') (* J[K] ~ let x = K' in J'[0] *)
+    K_cons j k ~ₖ K_let' k' <| ↑j'[0] |> (* J[K] ~ let x = K' in J'[0] *)
 with sim_val {A} : val A → val' A → Prop :=
 | sim_val_abs : ∀ e e', tm_abs e ~ₑ tm_abs' e' → val_abs e ~ᵥ val_abs' e'
+with sim_non {A} : non A → non' A → Prop :=
+| sim_non_ : ∀ p p', non_to_tm p ~ₑ non_to_tm' p' → p ~ₚ p'
 with sim_tm {A} : tm A → tm' A → Prop :=
-| sim_var  : ∀ a,    tm_var a ~ₑ tm_var' a
-| sim_abs  : ∀ e e', e ~ₑ e' → tm_abs e ~ₑ tm_abs' e'
-| sim_s_0  : ∀ e e', e ~ₑ e' → tm_s_0 e ~ₑ tm_s_0' e'
-| sim_app  : ∀ e1 e2 e1' e2', e1 ~ₑ e1' → e2 ~ₑ e2' → tm_app e1 e2 ~ₑ tm_app' e1' e2'
-| sim_dol  : ∀ e1 e2 e1' e2', e1 ~ₑ e1' → e2 ~ₑ e2' → tm_dol e1 e2 ~ₑ tm_dol' e1' e2'
+| sim_var  : ∀ a, <{ var a }> ~ₑ <| var a |>
+| sim_abs  : ∀ e e', e ~ₑ e' → <{ λ  e }> ~ₑ <| λ  e' |>
+| sim_s_0  : ∀ e e', e ~ₑ e' → <{ S₀ e }> ~ₑ <| S₀ e' |>
+| sim_app  : ∀ e1 e2 e1' e2', e1 ~ₑ e1' → e2 ~ₑ e2' → <{ e1   e2 }> ~ₑ <| e1'   e2' |>
+| sim_dol  : ∀ e1 e2 e1' e2', e1 ~ₑ e1' → e2 ~ₑ e2' → <{ e1 $ e2 }> ~ₑ <| e1' $ e2' |>
 (* | sim_plug : ∀ k k' e e', k ~ₖ k' → e ~ₑ e' → plugK k e ~ₑ plugK' k' e' *)
 | sim_plug : ∀ v v' k k' e e',
     k ~ₖ k' → e ~ₑ e' →
-    (* λ x. v $ K[0] ~ λ x. v' $ K'[0] *)
-    tm_abs  (tm_dol  (lift  (val_to_tm  v )) (plugK  (liftK  k ) (tm_var  None))) ~ₑ 
-    tm_abs' (tm_dol' (lift' (val_to_tm' v')) (plugK' (liftK' k') (tm_var' None)))
+    <{ λ {liftV  v } $ ↑k [0] }> ~ₑ <| λ {liftV' v'} $ ↑k'[0] |>
 where "e ~ₑ e'" := (sim_tm  e e')
 and   "v ~ᵥ v'" := (sim_val v v')
+and   "p ~ₚ p'" := (sim_non p p')
 and   "j ~ⱼ j'" := (sim_J   j j')
-and   "k ~ₖ k'" := (sim_K   k k').
+and   "k ~ₖ k'" := (sim_K   k k')
+and   "t ~ₜ t'" := (sim_T   t t').
 Global Hint Constructors sim_J : core.
 Global Hint Constructors sim_K : core.
+Global Hint Constructors sim_T : core.
 Global Hint Constructors sim_val : core.
+Global Hint Constructors sim_non : core.
 Global Hint Constructors sim_tm : core.
 
-Lemma lval_sim_inv : ∀ {A} (v : val A) (e' : tm' A),
+Reserved Notation "e ~ e'" (at level 40).
+Inductive sim_toplevel {A} : tm A → tm' A → Prop :=
+| sim_top_base : ∀ e e', e ~ₑ e' → e ~ e'
+| sim_top_cons : ∀ k k' t t' e e',
+    k ~ₖ k' → t ~ₜ t' → e ~ₑ e' → 
+    <{ k[t[e]] }> ~ <| k'[t'[e']] |>
+where "e ~ e'" := (sim_toplevel e e').
+Global Hint Constructors sim_toplevel : core.
+
+Lemma sim_val_inv : ∀ {A} (v : val A) (e' : tm' A),
   v ~ₑ e' → ∃ (v' : val' A), e' = v' /\ v ~ᵥ v'.
 Proof.
   intros. destruct v. inversion H; clear H; subst.
   exists (val_abs' e'0); auto.
-  exists (val_abs' <{ {lift' v'} $ {plugK' (liftK' k') <{ 0 }>'} }>'); split; auto.
+  exists (val_abs' <| {liftV' v'} $ ↑k'[0] |>); split; auto.
   constructor.
   eapply (sim_plug v v' k k'); eassumption.
 Qed.
 
+Lemma sim_non_inv : ∀ {A} (p : non A) (e' : tm' A),
+  p ~ₑ e' → ∃ (p' : non' A), e' = p' /\ p ~ₚ p'.
+Proof.
+  intros. destruct p; inversion H; clear H; subst.
+  exists (non_s_0' e'0); split; auto; repeat constructor; assumption.
+  exists (non_app' e1' e2'); split; auto; repeat constructor; assumption.
+  exists (non_dol' e1' e2'); split; auto; repeat constructor; assumption.
+Qed.
+
+Lemma sim_j_inv : ∀ (j : J ␀) e term',
+  <{ j[e] }> ~ₑ term' → ∃ j' e', j ~ⱼ j' /\ e ~ₑ e' /\ term' = <| j'[e'] |>.
+Proof.
+  intros. inversion H; clear H; subst;
+    try destruct a; 
+    destruct j; inversion H0; clear H0; subst; cbn in *;
+    try solve [repeat eexists; eauto].
+  apply sim_val_inv in H1 as [v' [Hvv Hv]]; subst.
+  repeat eexists; eauto.
+Qed.
+
+(* k[p] *)
+Lemma plug_k_steps_to_similar_k' : ∀ (k : K ␀) (p : non ␀) term',
+  <{ k [p] }> ~ₑ term' →
+  ∃ (k' : K' ␀) (p' : non' ␀),
+    term' -->'* <| k'[ p'] |> /\
+    k ~ₖ k' /\
+    p ~ₚ p'.
+Proof.
+  induction k; intros; cbn in *.
+  - apply sim_non_inv in H as [p' [H Hp]]; subst.
+    exists K_nil'; exists p'; auto.
+  - apply sim_j_inv in H as [j' [e' [Hj [Hke Hje]]]]; subst.
+    apply IHk in Hke as [k' [p'' [Hstep [Hk He]]]].
+    inversion He; clear He; subst. 
+    apply (non_when_steps_to_plug_non' _ _ T_nil') in Hstep as Haux. destruct Haux as [p' HH]. subst.
+    exists (K_let' k' <| ↑j'[0] |>). exists p''. cbn.
+    repeat split; auto.
+    apply (multi_contr' _ _ _ (contr_let' j' p')).
+    apply (multi_let'). apply Hstep.
+  Qed.
 (* v $ K[S₀ f. e] -->'* e [f := λ x. v $ K'[x]] *)
 (* Lemma aux :
   <{ {val_abs v} $ {plugK k <{ S₀ e }>} }> *)
